formal/dafny/CaveatSchema.dfy
@@ -10,11 +10,11 @@ module CaveatSchema {
   predicate Valid(s: Schema) {
     0 !in s.definitions &&
     (forall n | n in s.definitions :: s.definitions[n].booleanRoot && s.definitions[n].profile == 1 && |s.definitions[n].parameters| <= 32) &&
-    (forall relation | relation in s.allowances :: s.allowances[relation] <= s.definitions.Keys)
+    (forall relation | relation in s.allowances :: s.allowances[relation] - {0} <= s.definitions.Keys)
   }
 
   predicate Allowed(s: Schema, relation: nat, caveat: nat) {
-    caveat == 0 || (relation in s.allowances && caveat in s.allowances[relation])
+    relation in s.allowances && caveat in s.allowances[relation]
   }
 
   function Replace(current: Schema, expected: nat, candidate: Schema, retained: set<nat>): Replacement {
@@ -48,6 +48,11 @@ module CaveatSchema {
   lemma RelationMustAllowQualifiedCaveat(s: Schema, relation: nat, caveat: nat)
     requires caveat != 0 && (relation !in s.allowances || caveat !in s.allowances[relation])
     ensures !Allowed(s, relation, caveat)
+  {
+  }
+
+  lemma UnqualifiedRequiresPlainBranch(s: Schema, relation: nat)
+    ensures Allowed(s, relation, 0) <==> relation in s.allowances && 0 in s.allowances[relation]
   {
   }
 
